erasure/theories/EBeta.v
@@ -1,0 +1,120 @@
+From Coq Require Import List.
+From Coq Require Import String.
+From MetaCoq.Utils Require Import utils.
+From MetaCoq.Common Require Import BasicAst.
+From MetaCoq.Erasure Require Import EPrimitive EAst EAstUtils ELiftSubst EProgram.
+
+Definition map_subterms (f : term -> term) (t : term) : term :=
+  match t with
+  | tEvar n ts => tEvar n (map f ts)
+  | tLambda na body => tLambda na (f body)
+  | tLetIn na val body => tLetIn na (f val) (f body)
+  | tApp hd arg => tApp (f hd) (f arg)
+  | tCase p disc brs =>
+    tCase p (f disc) (map (on_snd f) brs)
+  | tProj p t => tProj p (f t)
+  | tFix def i => tFix (map (map_def f) def) i
+  | tCoFix def i => tCoFix (map (map_def f) def) i
+  | tPrim p => tPrim (map_prim f p)
+  | tLazy t => tLazy (f t)
+  | tForce t => tForce (f t)
+  | tConstruct ind n args => tConstruct ind n (map f args)
+  | t => t
+  end.
+
+Section betared.
+  Fixpoint decompose_lam (t : term) {struct t} : list name × term :=
+    match t with
+    | tLambda na B =>
+      let (ns, B0) := decompose_lam B in
+      (na :: ns, B0)
+    | _ => ([], t)
+    end.
+
+  Fixpoint beta_body (body : term) (args : list term) {struct args} : term :=
+    match args with
+    | [] => body
+    | a :: args =>
+        match body with
+        | tLambda na body => beta_body (body{0 := a}) args
+        | _ => mkApps body (a :: args)
+        end
+    end.
+
+  Fixpoint betared_aux (args : list term) (t : term) : term :=
+    match t with
+    | tApp hd arg => betared_aux (betared_aux [] arg :: args) hd
+    | tLambda na body =>
+      let b := betared_aux [] body in
+      beta_body (tLambda na b) args
+    | t => mkApps (map_subterms (betared_aux []) t) args
+    end.
+
+  Definition betared : term -> term := betared_aux [].
+
+  Definition betared_in_constant_body cst :=
+    {| cst_body := option_map betared (cst_body cst); |}.
+
+  Definition betared_in_decl d :=
+    match d with
+    | ConstantDecl cst => ConstantDecl (betared_in_constant_body cst)
+    | _ => d
+    end.
+
+End betared.
+
+Definition betared_env (Σ : global_declarations) : global_declarations :=
+  map (fun '(kn, decl) => (kn, betared_in_decl decl)) Σ.
+
+Definition betared_program (p : program) : program :=
+  (betared_env p.1, betared p.2).
+
+From MetaCoq.Erasure Require Import EProgram EWellformed EWcbvEval.
+From MetaCoq.Common Require Import Transform.
+
+Axiom trust_betared_wf :
+  forall efl : EEnvFlags,
+  WcbvFlags ->
+  forall (input : Transform.program _ term),
+  wf_eprogram efl input -> wf_eprogram efl (betared_program input).
+Axiom trust_betared_pres :
+  forall (efl : EEnvFlags) (wfl : WcbvFlags) (p : Transform.program _ term)
+  (v : term),
+  wf_eprogram efl p ->
+  eval_eprogram wfl p v ->
+  exists v' : term,
+  eval_eprogram wfl (betared_program p) v' /\ v' = betared v.
+
+Import Transform.
+
+Program Definition betared_transformation (efl : EEnvFlags) (wfl : WcbvFlags) :
+  Transform.t _ _ EAst.term EAst.term _ _
+    (eval_eprogram wfl) (eval_eprogram wfl) :=
+  {| name := "betared ";
+    transform p _ := betared_program p ;
+    pre p := wf_eprogram efl p ;
+    post p := wf_eprogram efl p ;
+    obseq p hp p' v v' := v' = betared v |}.
+
+Next Obligation.
+  now apply trust_betared_wf.
+Qed.
+Next Obligation.
+  now eapply trust_betared_pres.
+Qed.
+
+Import EProgram EGlobalEnv.
+
+#[global]
+Axiom betared_transformation_ext :
+  forall (efl : EEnvFlags) (wfl : WcbvFlags),
+  TransformExt.t (betared_transformation efl wfl)
+    (fun p p' => extends p.1 p'.1) (fun p p' => extends p.1 p'.1).
+
+#[global]
+Axiom betared_transformation_ext' :
+  forall (efl : EEnvFlags) (wfl : WcbvFlags),
+  TransformExt.t (betared_transformation efl wfl)
+    extends_eprogram extends_eprogram.
+
+
